src/Duplicate.v
@@ -10,21 +10,22 @@ Set Implicit Arguments.
 Set Asymmetric Patterns.
 
 Section Duplicate.
-  Variable m: Modules.
+  Variable m: nat -> Modules.
 
   Fixpoint duplicate n :=
     match n with
-    | O => specializeMod m O
-    | S n' => ConcatMod (specializeMod m n) (duplicate n')
+    | O => specializeMod (m O) O
+    | S n' => ConcatMod (specializeMod (m n) n) (duplicate n')
     end.
 
 End Duplicate.
 
 Section DuplicateFacts.
+  Variable m: nat -> Modules.
 
   Lemma duplicate_ModEquiv:
-    forall ty1 ty2 m n,
-      ModEquiv ty1 ty2 m ->
+    forall ty1 ty2 n,
+      (forall iv, ModEquiv ty1 ty2 (m iv)) ->
       ModEquiv ty1 ty2 (duplicate m n).
   Proof.
     induction n; simpl; intros;
@@ -34,8 +35,8 @@ Section DuplicateFacts.
   Qed.
 
   Lemma duplicate_validRegsModules:
-    forall m n,
-      ValidRegsModules type m ->
+    forall n,
+      (forall iv, ValidRegsModules type (m iv)) ->
       ValidRegsModules type (duplicate m n).
   Proof.
     induction n; simpl; intros.
@@ -45,87 +46,85 @@ Section DuplicateFacts.
   Qed.
 
   Lemma duplicate_dom_indexed:
-    forall m,
-      Specializable m ->
-      forall s n,
-        In s (spDom (duplicate m n)) ->
-        exists t i, s = t __ i /\ i < S n.
+    (forall iv, Specializable (m iv)) ->
+    forall s n ,
+      In s (spDom (duplicate m n)) ->
+      exists t i, s = t __ i /\ i < S n.
   Proof.
     induction n; simpl; intros.
-    - pose proof (specializeMod_dom_indexed H _ _ H0); dest; subst.
+    - pose proof (specializeMod_dom_indexed (H 0) _ _ H0); dest; subst.
       do 2 eexists; eauto.
     - apply spDom_in in H0; destruct H0.
-      + pose proof (specializeMod_dom_indexed H _ _ H0); dest; subst.
+      + pose proof (specializeMod_dom_indexed (H (S n)) _ _ H0); dest; subst.
         do 2 eexists; eauto.
       + specialize (IHn H0); dest; subst.
         do 2 eexists; eauto.
   Qed.
 
   Lemma duplicate_specializeMod_disj_regs:
-    forall m,
-      Specializable m ->
-      forall n ln,
-        ln > n ->
-        DisjList (namesOf (getRegInits (specializeMod m ln)))
-                 (namesOf (getRegInits (duplicate m n))).
+    (forall iv, Specializable (m iv)) ->
+    forall n ln iv,
+      ln > n ->
+      DisjList (namesOf (getRegInits (specializeMod (m iv) ln)))
+               (namesOf (getRegInits (duplicate m n))).
   Proof.
     induction n; simpl; intros.
-    - apply specializable_disj_regs; auto; omega.
+    - apply specializeMod_disj_regs_different_indices; auto; omega.
     - unfold namesOf in *.
       rewrite map_app.
       apply DisjList_comm, DisjList_app_4.
-      + apply specializable_disj_regs; auto; omega.
+      + apply specializeMod_disj_regs_different_indices; auto; omega.
       + apply DisjList_comm, IHn; omega.
   Qed.
 
   Lemma duplicate_specializeMod_disj_defs:
-    forall m,
-      Specializable m ->
-      forall n ln,
-        ln > n ->
-        DisjList (getDefs (specializeMod m ln))
-                 (getDefs (duplicate m n)).
+    (forall iv, Specializable (m iv)) ->
+    forall n ln iv,
+      ln > n ->
+      DisjList (getDefs (specializeMod (m iv) ln))
+               (getDefs (duplicate m n)).
   Proof.
     induction n; simpl; intros.
-    - apply specializable_disj_defs; auto; omega.
+    - apply specializeMod_disj_defs_different_indices; auto; omega.
     - apply DisjList_comm.
-      apply DisjList_SubList with (l1:= app (getDefs (specializeMod m (S n)))
-                                            (getDefs (duplicate m n))).
+      apply DisjList_SubList with
+      (l1:= app (getDefs (specializeMod (m (S n)) (S n)))
+                (getDefs (duplicate m n))).
       + unfold SubList; intros.
         apply getDefs_in in H1; destruct H1;
           apply in_or_app; auto.
       + apply DisjList_app_4.
-        * apply specializable_disj_defs; auto; omega.
+        * apply specializeMod_disj_defs_different_indices; auto; omega.
         * apply DisjList_comm, IHn; omega.
   Qed.
 
   Lemma duplicate_specializeMod_disj_calls:
-    forall m,
-      Specializable m ->
-      forall n ln,
-        ln > n ->
-        DisjList (getCalls (specializeMod m ln))
-                 (getCalls (duplicate m n)).
+    (forall iv, Specializable (m iv)) ->
+    forall n ln iv,
+      ln > n ->
+      DisjList (getCalls (specializeMod (m iv) ln))
+               (getCalls (duplicate m n)).
   Proof.
     induction n; simpl; intros.
-    - apply specializable_disj_calls; auto; omega.
+    - apply specializeMod_disj_calls_different_indices; auto; omega.
     - apply DisjList_comm.
-      apply DisjList_SubList with (l1:= app (getCalls (specializeMod m (S n)))
-                                            (getCalls (duplicate m n))).
+      apply DisjList_SubList with
+      (l1:= app (getCalls (specializeMod (m (S n)) (S n)))
+                (getCalls (duplicate m n))).
       + unfold SubList; intros.
         apply getCalls_in in H1; destruct H1;
           apply in_or_app; auto.
       + apply DisjList_app_4.
-        * apply specializable_disj_calls; auto; omega.
+        * apply specializeMod_disj_calls_different_indices; auto; omega.
         * apply DisjList_comm, IHn; omega.
   Qed.
   
   Lemma duplicate_disj_regs:
     forall m1 m2,
-      Specializable m1 ->
-      Specializable m2 ->
-      DisjList (namesOf (getRegInits m1))
-               (namesOf (getRegInits m2)) ->
+      (forall iv1, Specializable (m1 iv1)) ->
+      (forall iv2, Specializable (m2 iv2)) ->
+      (forall iv1 iv2, DisjList (namesOf (getRegInits (m1 iv1)))
+                                (namesOf (getRegInits (m2 iv2)))) ->
       forall n,
         DisjList (namesOf (getRegInits (duplicate m1 n)))
                  (namesOf (getRegInits (duplicate m2 n))).
@@ -135,73 +134,90 @@ Section DuplicateFacts.
     - unfold namesOf; do 2 rewrite map_app; apply DisjList_app_4.
       + apply DisjList_comm, DisjList_app_4.
         * apply DisjList_comm, specializeMod_disj_regs_2; auto.
-        * clear IHn; generalize (S n); intros; induction n; simpl.
+        * clear IHn.
+          assert (n < S n) by omega.
+          generalize dependent (S n); intros.
+          induction n; simpl; intros.
           { apply DisjList_comm, specializeMod_disj_regs_2; auto. }
-          { rewrite map_app; apply DisjList_app_4; auto.
-            apply DisjList_comm, specializeMod_disj_regs_2; auto.
+          { rewrite map_app; apply DisjList_app_4.
+            { apply DisjList_comm, specializeMod_disj_regs_2; auto. }
+            { apply IHn; omega. }
           }
       + apply DisjList_comm, DisjList_app_4.
-        * clear IHn; generalize (S n); intros; induction n; simpl.
+        * clear IHn.
+          assert (n < S n) by omega.
+          generalize dependent (S n); intros.
+          induction n; simpl; intros.
           { apply DisjList_comm, specializeMod_disj_regs_2; auto. }
           { rewrite map_app; apply DisjList_comm, DisjList_app_4.
             { apply specializeMod_disj_regs_2; auto. }
-            { apply DisjList_comm; auto. }
+            { apply DisjList_comm; auto.
+              apply IHn; omega.
+            }
           }
-        * apply DisjList_comm; auto.
+        * apply DisjList_comm, IHn.
   Qed.
 
   Lemma duplicate_noninteracting:
-    forall m,
-      Specializable m ->
-      forall n ln,
-        ln > n ->
-        NonInteracting (specializeMod m ln)
+    (forall iv, Specializable (m iv)) ->
+    forall n ln,
+      ln > n ->
+      forall iv,
+        NonInteracting (specializeMod (m iv) ln)
                        (duplicate m n).
   Proof.
     induction n; simpl; intros.
-    - apply specializable_noninteracting; auto; omega.
+    - apply specializable_noninteracting_2; auto; omega.
     - unfold NonInteracting in *.
       assert (ln > n) by omega; specialize (IHn _ H1); clear H1; dest.
       split.
       + apply DisjList_comm.
-        apply DisjList_SubList with (l1:= app (getCalls (specializeMod m (S n)))
-                                              (getCalls (duplicate m n))).
+        apply DisjList_SubList with
+        (l1:= app (getCalls (specializeMod (m (S n)) (S n)))
+                  (getCalls (duplicate m n))).
         * unfold SubList; intros.
-          apply getCalls_in in H3.
+          apply getCalls_in in H1.
           apply in_or_app; auto.
         * apply DisjList_app_4.
-          { pose proof (specializable_noninteracting H).
-            apply H3; omega.
+          { pose proof (specializable_noninteracting_2 (H (S n)) (H iv)).
+            apply H1; omega.
           }
-          { apply DisjList_comm; auto. }
+          { specialize (IHn iv); dest.
+            apply DisjList_comm; auto.
+          }
       + apply DisjList_comm.
-        apply DisjList_SubList with (l1:= app (getDefs (specializeMod m (S n)))
-                                              (getDefs (duplicate m n))).
+        apply DisjList_SubList with
+        (l1:= app (getDefs (specializeMod (m (S n)) (S n)))
+                  (getDefs (duplicate m n))).
         * unfold SubList; intros.
-          apply getDefs_in in H3.
+          apply getDefs_in in H1.
           apply in_or_app; auto.
         * apply DisjList_app_4.
-          { pose proof (specializable_noninteracting H).
-            apply H3; omega.
+          { pose proof (specializable_noninteracting_2 (H (S n)) (H iv)).
+            apply H1; omega.
           }
-          { apply DisjList_comm; auto. }
+          { specialize (IHn iv); dest.
+            apply DisjList_comm; auto.
+          }
   Qed.
 
   Lemma duplicate_regs_NoDup:
-    forall m (Hsp: Specializable m) n,
-      NoDup (namesOf (getRegInits m)) ->
+    forall (Hsp: forall iv, Specializable (m iv)) n,
+      (forall iv, NoDup (namesOf (getRegInits (m iv)))) ->
       NoDup (namesOf (getRegInits (duplicate m n))).
   Proof.
     induction n; simpl; intros; [apply specializeMod_regs_NoDup; auto|].
     unfold namesOf in *; simpl in *.
     rewrite map_app; apply NoDup_DisjList; auto.
-    - apply specializeMod_regs_NoDup; auto.
+    - apply specializeMod_regs_NoDup, H; auto.
     - apply duplicate_specializeMod_disj_regs; auto.
   Qed.
 
   Lemma getRegInits_duplicate_nil:
-    forall m n,
-      Specializable m -> getRegInits m = nil -> getRegInits (duplicate m n) = nil.
+    forall n,
+      (forall iv, Specializable (m iv)) ->
+      (forall iv, getRegInits (m iv) = nil) ->
+      getRegInits (duplicate m n) = nil.
   Proof.
     intros.
     match goal with
@@ -210,19 +226,22 @@ Section DuplicateFacts.
     { intros; unfold namesOf in H1; eapply map_eq_nil; eauto. }
     apply Hm; clear Hm.
     
-    induction n.
-    - simpl; rewrite specializeMod_regs; auto.
+    induction n; simpl; intros.
+    - rewrite specializeMod_regs; auto.
       rewrite H0; reflexivity.
-    - simpl; rewrite namesOf_app.
+    - rewrite namesOf_app.
       rewrite IHn; rewrite app_nil_r.
       rewrite specializeMod_regs; auto.
       rewrite H0; reflexivity.
   Qed.
 
   Lemma getDefs_duplicate_nil:
-    forall m n, Specializable m -> getDefs m = nil -> getDefs (duplicate m n) = nil.
+    (forall iv, Specializable (m iv)) ->
+    (forall iv, getDefs (m iv) = nil) ->
+    forall n,
+      getDefs (duplicate m n) = nil.
   Proof.
-    intros; induction n; simpl.
+    induction n; simpl; intros.
     - rewrite specializeMod_defs; auto.
       rewrite H0; reflexivity.
     - rewrite getDefs_app.
@@ -232,21 +251,26 @@ Section DuplicateFacts.
   Qed.
 
   Lemma getDefsBodies_duplicate_nil:
-    forall m n, Specializable m -> getDefsBodies m = nil -> getDefsBodies (duplicate m n) = nil.
+    (forall iv, Specializable (m iv)) ->
+    (forall iv, getDefsBodies (m iv) = nil) ->
+    forall n,
+      getDefsBodies (duplicate m n) = nil.
   Proof.
     intros.
-    assert (getDefs m = nil) by (unfold getDefs; rewrite H0; reflexivity).
-    apply getDefs_duplicate_nil with (n:= n) in H1; auto.
+    assert (forall iv, getDefs (m iv) = nil) by (intros; unfold getDefs; rewrite H0; reflexivity).
+    eapply getDefs_duplicate_nil with (n:= n) in H1; eauto.
     eapply map_eq_nil with (f:= @attrName _); eauto.
   Qed.
 
   Lemma getRules_duplicate_in:
-    forall m rn rb i n,
-      Specializable m ->
-      In (rn :: rb)%struct (getRules m) ->
-      le i n ->
-      In ((rn __ i) :: (fun ty => (Renaming.renameAction (specializer m i) (rb ty))))%struct
-         (getRules (duplicate m n)).
+    forall rn rb i,
+      (forall iv, Specializable (m iv)) ->
+      In (rn :: rb)%struct (getRules (m i)) ->
+      forall n,
+        i <= n ->
+        In ((rn __ i)
+              :: (fun ty => (Renaming.renameAction (specializer (m i) i) (rb ty))))%struct
+           (getRules (duplicate m n)).
   Proof.
     induction n; simpl; intros.
     - inv H1; apply specializeMod_rules_in; auto.
@@ -255,549 +279,588 @@ Section DuplicateFacts.
       apply specializeMod_rules_in; auto.
   Qed.
 
-  Section TwoModules1.
-    Variables (m1 m2: Modules).
-    Hypotheses (Hsp1: Specializable m1)
-               (Hsp2: Specializable m2)
-               (Hequiv1: ModEquiv type typeUT m1)
-               (Hequiv2: ModEquiv type typeUT m2)
-               (Hvr1: ValidRegsModules type m1)
-               (Hvr2: ValidRegsModules type m2)
-               (Hexts: SubList (getExtMeths m1) (getExtMeths m2)).
+End DuplicateFacts.
 
-    Lemma specializer_equiv:
-      forall {A} (m: M.t A),
-        M.KeysSubset m (spDom m1) ->
-        M.KeysSubset m (spDom m2) ->
-        forall i,
-          renameMap (specializer m1 i) m = renameMap (specializer m2 i) m.
-    Proof. intros; do 2 (rewrite specializer_map; auto). Qed.
+Section TwoModules1.
+  Variables (m1 m2: Modules).
+  Hypotheses (Hsp1: Specializable m1)
+             (Hsp2: Specializable m2)
+             (Hequiv1: ModEquiv type typeUT m1)
+             (Hequiv2: ModEquiv type typeUT m2)
+             (Hvr1: ValidRegsModules type m1)
+             (Hvr2: ValidRegsModules type m2)
+             (Hexts: SubList (getExtMeths m1) (getExtMeths m2)).
 
-    Lemma specializeMod_defCallSub:
+  Lemma specializer_equiv:
+    forall {A} (m: M.t A),
+      M.KeysSubset m (spDom m1) ->
+      M.KeysSubset m (spDom m2) ->
       forall i,
-        DefCallSub m1 m2 ->
-        DefCallSub (specializeMod m1 i) (specializeMod m2 i).
-    Proof.
-      unfold DefCallSub; intros; dest; split.
-      - do 2 rewrite specializeMod_defs by assumption.
-        apply SubList_map; auto.
-      - do 2 rewrite specializeMod_calls by assumption.
-        apply SubList_map; auto.
-    Qed.
+        renameMap (specializer m1 i) m = renameMap (specializer m2 i) m.
+  Proof. intros; do 2 (rewrite specializer_map; auto). Qed.
 
-    Lemma duplicate_defCallSub:
-      forall n,
-        DefCallSub m1 m2 ->
-        DefCallSub (duplicate m1 n) (duplicate m2 n).
-    Proof.
-      induction n; simpl; intros.
-      - apply specializeMod_defCallSub; auto.
-      - apply DefCallSub_modular; auto.
-        apply specializeMod_defCallSub; auto.
-    Qed.
+  Lemma specializeMod_defCallSub:
+    forall i,
+      DefCallSub m1 m2 ->
+      DefCallSub (specializeMod m1 i) (specializeMod m2 i).
+  Proof.
+    unfold DefCallSub; intros; dest; split.
+    - do 2 rewrite specializeMod_defs by assumption.
+      apply SubList_map; auto.
+    - do 2 rewrite specializeMod_calls by assumption.
+      apply SubList_map; auto.
+  Qed.
 
-    Lemma specializer_two_comm:
-      forall (m: MethsT),
-        M.KeysSubset m (getExtMeths m1) ->
-        forall i,
-          m = renameMap (specializer m2 i) (renameMap (specializer m1 i) m).
-    Proof.
-      intros.
-      replace (renameMap (specializer m1 i) m) with (renameMap (specializer m2 i) m).
-      - rewrite renameMapFInvG; auto.
-        + apply specializer_bijective.
-          apply specializable_disj_dom_img; auto.
-        + apply specializer_bijective.
-          apply specializable_disj_dom_img; auto.
-      - apply eq_sym, specializer_equiv.
-        + eapply M.KeysSubset_SubList; eauto.
-          pose proof (getExtMeths_meths m1).
-          apply SubList_trans with (l2:= app (getDefs m1) (getCalls m1)); auto.
-          apply SubList_app_3; [apply spDom_defs|apply spDom_calls].
-        + apply M.KeysSubset_SubList with (d2:= getExtMeths m2) in H; auto.
-          eapply M.KeysSubset_SubList; eauto.
-          pose proof (getExtMeths_meths m2).
-          apply SubList_trans with (l2:= app (getDefs m2) (getCalls m2)); auto.
-          apply SubList_app_3; [apply spDom_defs|apply spDom_calls].
-    Qed.
+  Lemma specializer_two_comm:
+    forall (m: MethsT),
+      M.KeysSubset m (getExtMeths m1) ->
+      forall i,
+        m = renameMap (specializer m2 i) (renameMap (specializer m1 i) m).
+  Proof.
+    intros.
+    replace (renameMap (specializer m1 i) m) with (renameMap (specializer m2 i) m).
+    - rewrite renameMapFInvG; auto.
+      + apply specializer_bijective.
+        apply specializable_disj_dom_img; auto.
+      + apply specializer_bijective.
+        apply specializable_disj_dom_img; auto.
+    - apply eq_sym, specializer_equiv.
+      + eapply M.KeysSubset_SubList; eauto.
+        pose proof (getExtMeths_meths m1).
+        apply SubList_trans with (l2:= app (getDefs m1) (getCalls m1)); auto.
+        apply SubList_app_3; [apply spDom_defs|apply spDom_calls].
+      + apply M.KeysSubset_SubList with (d2:= getExtMeths m2) in H; auto.
+        eapply M.KeysSubset_SubList; eauto.
+        pose proof (getExtMeths_meths m2).
+        apply SubList_trans with (l2:= app (getDefs m2) (getCalls m2)); auto.
+        apply SubList_app_3; [apply spDom_defs|apply spDom_calls].
+  Qed.
 
-    Lemma duplicate_traceRefines:
-      forall n,
-        traceRefines (liftToMap1 (@idElementwise _)) m1 m2 ->
-        traceRefines (liftToMap1 (@idElementwise _)) (duplicate m1 n) (duplicate m2 n).
-    Proof.
-      induction n; simpl; intros.
-      - apply specialized_2 with (i:= O); auto.
+End TwoModules1.
+
+Section DuplicateTwoModules1.
+  Variables (m1 m2: nat -> Modules).
+  Hypotheses (Hsp1: forall iv, Specializable (m1 iv))
+             (Hsp2: forall iv, Specializable (m2 iv))
+             (Hequiv1: forall iv, ModEquiv type typeUT (m1 iv))
+             (Hequiv2: forall iv, ModEquiv type typeUT (m2 iv))
+             (Hvr1: forall iv, ValidRegsModules type (m1 iv))
+             (Hvr2: forall iv, ValidRegsModules type (m2 iv))
+             (Hexts: forall iv1 iv2, SubList (getExtMeths (m1 iv1)) (getExtMeths (m2 iv2))).
+
+  Lemma duplicate_defCallSub:
+    forall n,
+      (forall i, DefCallSub (m1 i) (m2 i)) ->
+      DefCallSub (duplicate m1 n) (duplicate m2 n).
+  Proof.
+    induction n; simpl; intros.
+    - apply specializeMod_defCallSub; auto.
+    - apply DefCallSub_modular.
+      + apply specializeMod_defCallSub; auto.
+      + apply IHn; auto.
+  Qed.
+
+  Lemma duplicate_traceRefines:
+    forall n,
+      (forall i, traceRefines (liftToMap1 (@idElementwise _)) (m1 i) (m2 i)) ->
+      traceRefines (liftToMap1 (@idElementwise _))
+                   (duplicate m1 n)
+                   (duplicate m2 n).
+  Proof.
+    induction n; simpl; intros.
+    - apply specialized_2 with (i:= O); auto.
+      specialize (H 0).
+      eapply traceRefines_label_map; eauto using H.
+      clear - Hsp1 Hsp2 Hexts; unfold EquivalentLabelMap; intros.
+      rewrite idElementwiseId; unfold id; simpl.
+      unfold liftPRename; simpl.
+      apply specializer_two_comm; auto.
+
+    - apply traceRefines_modular_noninteracting; auto.
+      + apply specializeMod_ModEquiv; auto.
+      + apply specializeMod_ModEquiv; auto.
+      + apply duplicate_ModEquiv; auto.
+      + apply duplicate_ModEquiv; auto.
+      + apply duplicate_specializeMod_disj_regs; auto.
+      + apply duplicate_specializeMod_disj_regs; auto.
+      + pose proof (duplicate_validRegsModules m1 (S n) Hvr1); auto.
+      + pose proof (duplicate_validRegsModules m2 (S n) Hvr2); auto.
+      + apply duplicate_specializeMod_disj_defs; auto.
+      + apply duplicate_specializeMod_disj_calls; auto.
+      + apply duplicate_specializeMod_disj_defs; auto.
+      + apply duplicate_specializeMod_disj_calls; auto.
+      + apply duplicate_noninteracting; auto.
+      + apply duplicate_noninteracting; auto.
+      + apply specialized_2 with (i:= S n); auto.
+        specialize (H (S n)).
         eapply traceRefines_label_map; eauto using H.
         clear - Hsp1 Hsp2 Hexts; unfold EquivalentLabelMap; intros.
         rewrite idElementwiseId; unfold id; simpl.
         unfold liftPRename; simpl.
         apply specializer_two_comm; auto.
+  Qed.
 
-      - apply traceRefines_modular_noninteracting; auto.
-        + apply specializeMod_ModEquiv; auto.
-        + apply specializeMod_ModEquiv; auto.
-        + apply duplicate_ModEquiv; auto.
-        + apply duplicate_ModEquiv; auto.
-        + apply duplicate_specializeMod_disj_regs; auto.
-        + apply duplicate_specializeMod_disj_regs; auto.
-        + pose proof (duplicate_validRegsModules m1 (S n) Hvr1); auto.
-        + pose proof (duplicate_validRegsModules m2 (S n) Hvr2); auto.
-        + apply duplicate_specializeMod_disj_defs; auto.
-        + apply duplicate_specializeMod_disj_calls; auto.
-        + apply duplicate_specializeMod_disj_defs; auto.
-        + apply duplicate_specializeMod_disj_calls; auto.
-        + apply duplicate_noninteracting; auto.
-        + apply duplicate_noninteracting; auto.
-        + apply specialized_2 with (i:= S n); auto.
-          eapply traceRefines_label_map; eauto using H.
-          clear - Hsp1 Hsp2 Hexts; unfold EquivalentLabelMap; intros.
-          rewrite idElementwiseId; unfold id; simpl.
-          unfold liftPRename; simpl.
-          apply specializer_two_comm; auto.
-    Qed.
+End DuplicateTwoModules1.
 
-  End TwoModules1.
+Section TwoModules2.
+  Variables (m1 m2: Modules).
+  Hypotheses (Hsp1: Specializable m1)
+             (Hsp2: Specializable m2)
+             (Hequiv1: ModEquiv type typeUT m1)
+             (Hequiv2: ModEquiv type typeUT m2)
+             (Hvr1: ValidRegsModules type m1)
+             (Hvr2: ValidRegsModules type m2).
 
-  Section TwoModules2.
-    Variables (m1 m2: Modules).
-    Hypotheses (Hsp1: Specializable m1)
-               (Hsp2: Specializable m2)
-               (Hequiv1: ModEquiv type typeUT m1)
-               (Hequiv2: ModEquiv type typeUT m2)
-               (Hvr1: ValidRegsModules type m1)
-               (Hvr2: ValidRegsModules type m2).
+  Variable (ds: string). (* a single label to drop *)
 
-    Variable (ds: string). (* a single label to drop *)
+  Hypothesis (Hexts: SubList (filter (fun s => negb (string_eq s ds)) (getExtMeths m1))
+                             (getExtMeths m2)).
 
-    Hypothesis (Hexts: SubList (filter (fun s => negb (string_eq s ds)) (getExtMeths m1))
-                               (getExtMeths m2)).
+  Lemma specializeMod_traceRefines_drop:
+    forall i,
+      (m1 <<=[dropP ds] m2) ->
+      (specializeMod m1 i <<=[dropI ds i] specializeMod m2 i).
+  Proof.
+    intros.
+    apply specialized_2; auto.
+    apply traceRefines_label_map with (p:= liftToMap1 (dropP ds)); auto.
 
-    Lemma specializeMod_traceRefines_drop:
-      forall i,
-        (m1 <<=[dropP ds] m2) ->
-        (specializeMod m1 i <<=[dropI ds i] specializeMod m2 i).
-    Proof.
-      intros.
-      apply specialized_2; auto.
-      apply traceRefines_label_map with (p:= liftToMap1 (dropP ds)); auto.
+    clear -Hsp1 Hsp2 Hexts.
+    unfold EquivalentLabelMap; intros.
 
-      clear -Hsp1 Hsp2 Hexts.
-      unfold EquivalentLabelMap; intros.
+    unfold liftPRename.
 
-      unfold liftPRename.
-
-      assert (renameMap (specializer m2 i) ((liftToMap1 (dropP ds)) m) =
-              liftToMap1 (dropI ds i) (renameMap (specializer m1 i) m)).
-      { rewrite specializer_map with (m:= m1); auto;
+    assert (renameMap (specializer m2 i) ((liftToMap1 (dropP ds)) m) =
+            liftToMap1 (dropI ds i) (renameMap (specializer m1 i) m)).
+    { rewrite specializer_map with (m:= m1); auto;
         [|eapply M.KeysSubset_SubList; eauto; apply spDom_getExtMeths].
-        rewrite specializer_map with (m:= m2); auto;
-          [|apply M.KeysSubset_SubList with (d1:= getExtMeths m2); [|apply spDom_getExtMeths];
-            eapply M.KeysSubset_SubList; eauto;
-            apply dropP_KeysSubset; auto].
+      rewrite specializer_map with (m:= m2); auto;
+        [|apply M.KeysSubset_SubList with (d1:= getExtMeths m2); [|apply spDom_getExtMeths];
+          eapply M.KeysSubset_SubList; eauto;
+          apply dropP_KeysSubset; auto].
 
-        clear; M.ext y.
-        rewrite liftToMap1_find.
-        remember (M.find y (renameMap (spf i) m)) as yiv; destruct yiv.
-        - apply eq_sym, renameFind2' in Heqyiv; [|apply spf_onto].
-          dest; subst; rewrite <-renameMapFind; [|apply spf_onto].
-          rewrite liftToMap1_find, H0.
-          unfold dropP, dropI.
-          remember (string_eq x ds) as xds; destruct xds.
-          + apply string_eq_dec_eq in Heqxds; subst.
-            rewrite string_eq_true; reflexivity.
-          + apply string_eq_dec_neq in Heqxds.
-            remember (string_eq (spf i x) (ds __ i)) as xdsi; destruct xdsi; auto.
-            apply string_eq_dec_eq, spf_onto in Heqxdsi.
-            elim Heqxds; auto.
-        - remember (M.find y (renameMap (spf i) (liftToMap1 (dropP ds) m))) as ypv;
-            destruct ypv; auto.
-          exfalso; apply eq_sym, renameFind2' in Heqypv; [|apply spf_onto].
-          dest; subst.
-          rewrite <-renameMapFind in Heqyiv; [|apply spf_onto].
-          rewrite liftToMap1_find in H0.
-          rewrite <-Heqyiv in H0; inv H0.
-      }
+      clear; M.ext y.
+      rewrite liftToMap1_find.
+      remember (M.find y (renameMap (spf i) m)) as yiv; destruct yiv.
+      - apply eq_sym, renameFind2' in Heqyiv; [|apply spf_onto].
+        dest; subst; rewrite <-renameMapFind; [|apply spf_onto].
+        rewrite liftToMap1_find, H0.
+        unfold dropP, dropI.
+        remember (string_eq x ds) as xds; destruct xds.
+        + apply string_eq_dec_eq in Heqxds; subst.
+          rewrite string_eq_true; reflexivity.
+        + apply string_eq_dec_neq in Heqxds.
+          remember (string_eq (spf i x) (ds __ i)) as xdsi; destruct xdsi; auto.
+          apply string_eq_dec_eq, spf_onto in Heqxdsi.
+          elim Heqxds; auto.
+      - remember (M.find y (renameMap (spf i) (liftToMap1 (dropP ds) m))) as ypv;
+          destruct ypv; auto.
+        exfalso; apply eq_sym, renameFind2' in Heqypv; [|apply spf_onto].
+        dest; subst.
+        rewrite <-renameMapFind in Heqyiv; [|apply spf_onto].
+        rewrite liftToMap1_find in H0.
+        rewrite <-Heqyiv in H0; inv H0.
+    }
 
-      rewrite <-H0.
-      rewrite <-specializer_two_comm with (m1:= m2) (m2:= m2) (i:= i); auto.
-      - apply SubList_refl.
-      - eapply M.KeysSubset_SubList; eauto.
-        apply dropP_KeysSubset; auto.
-    Qed.
+    rewrite <-H0.
+    rewrite <-specializer_two_comm with (m1:= m2) (m2:= m2) (i:= i); auto.
+    - apply SubList_refl.
+    - eapply M.KeysSubset_SubList; eauto.
+      apply dropP_KeysSubset; auto.
+  Qed.
 
-    Lemma equivalentLabelMapElem_dropI_dropN:
-      forall n t (Ht: t > n),
-        EquivalentLabelMapElem (dropI ds t) (compLabelMaps (dropI ds t) (dropN ds n))
-                               (getExtMeths (specializeMod m1 t)).
-    Proof.
-      unfold EquivalentLabelMapElem; intros.
-      induction n.
-      - simpl; unfold compLabelMaps, dropI.
-        destruct (string_eq _ (ds __ t)).
-        + destruct (string_eq _ (ds __ 0)); auto.
-        + remember (string_eq _ _) as sv; destruct sv; auto.
-          exfalso; apply string_eq_dec_eq in Heqsv; subst.
-          apply spDom_getExtMeths in H.
-          apply specializeMod_dom_indexed in H; auto; dest.
-          apply withIndex_index_eq in H; dest; omega.
-      - simpl; assert (t > n) by omega; specialize (IHn H0); clear H0.
-        rewrite IHn; clear IHn.
-        unfold dropI, compLabelMaps.
-        remember (dropN ds n s v) as nv; destruct nv; auto.
-        destruct (string_eq s (ds __ t)).
-        + destruct (string_eq _ _); auto.
-        + remember (string_eq _ _) as sn; destruct sn; auto.
-          exfalso; apply string_eq_dec_eq in Heqsn; subst.
-          apply spDom_getExtMeths in H.
-          apply specializeMod_dom_indexed in H; auto; dest.
-          apply withIndex_index_eq in H; dest; omega.
-    Qed.
-
-    Lemma equivalentLabelMapElem_dropN_dropI:
-      forall n t (Ht: t > n),
-        EquivalentLabelMapElem (dropN ds n) (compLabelMaps (dropI ds t) (dropN ds n))
-                               (getExtMeths (duplicate m1 n)).
-    Proof.
-      unfold EquivalentLabelMapElem; intros.
-      induction n.
-      - simpl; unfold compLabelMaps, dropI.
-        destruct (string_eq _ (ds __ 0)); auto.
-        remember (string_eq _ _) as st; destruct st; auto.
-        apply string_eq_dec_eq in Heqst; subst.
-        simpl in H.
+  Lemma equivalentLabelMapElem_dropI_dropN:
+    forall n t (Ht: t > n),
+      EquivalentLabelMapElem (dropI ds t) (compLabelMaps (dropI ds t) (dropN ds n))
+                             (getExtMeths (specializeMod m1 t)).
+  Proof.
+    unfold EquivalentLabelMapElem; intros.
+    induction n.
+    - simpl; unfold compLabelMaps, dropI.
+      destruct (string_eq _ (ds __ t)).
+      + destruct (string_eq _ (ds __ 0)); auto.
+      + remember (string_eq _ _) as sv; destruct sv; auto.
+        exfalso; apply string_eq_dec_eq in Heqsv; subst.
         apply spDom_getExtMeths in H.
         apply specializeMod_dom_indexed in H; auto; dest.
         apply withIndex_index_eq in H; dest; omega.
-      - simpl; assert (t > n) by omega; specialize (IHn H0); clear H0.
-        simpl in H.
-        apply getExtMeths_in in H; destruct H.
-        + clear IHn.
-          unfold dropI, compLabelMaps.
-          destruct (dropN ds n s v); auto.
-          destruct (string_eq _ (ds __ (S n))); auto.
-          remember (string_eq _ _) as st; destruct st; auto.
-          exfalso; apply string_eq_dec_eq in Heqst; subst.
-          apply spDom_getExtMeths in H.
-          apply specializeMod_dom_indexed in H; auto; dest.
-          apply withIndex_index_eq in H; dest; omega.
-        + specialize (IHn H).
-          unfold compLabelMaps.
-          rewrite IHn; clear IHn.
-          unfold compLabelMaps.
-          destruct (dropN ds n s v); auto.
-          destruct (dropI ds t s s0); auto.
-          destruct (dropI ds (S n) s s1); auto.
-          unfold dropI; remember (string_eq _ _) as st; destruct st; auto.
-          exfalso; apply string_eq_dec_eq in Heqst; subst.
-          apply spDom_getExtMeths in H.
-          apply duplicate_dom_indexed in H; auto; dest.
-          apply withIndex_index_eq in H; dest; omega.
-    Qed.
+    - simpl; assert (t > n) by omega; specialize (IHn H0); clear H0.
+      rewrite IHn; clear IHn.
+      unfold dropI, compLabelMaps.
+      remember (dropN ds n s v) as nv; destruct nv; auto.
+      destruct (string_eq s (ds __ t)).
+      + destruct (string_eq _ _); auto.
+      + remember (string_eq _ _) as sn; destruct sn; auto.
+        exfalso; apply string_eq_dec_eq in Heqsn; subst.
+        apply spDom_getExtMeths in H.
+        apply specializeMod_dom_indexed in H; auto; dest.
+        apply withIndex_index_eq in H; dest; omega.
+  Qed.
 
-    Lemma duplicate_traceRefines_drop:
-      forall n,
-        (m1 <<=[dropP ds] m2) ->
-        (duplicate m1 n <<=[dropN ds n] duplicate m2 n).
-    Proof.
-      induction n; simpl; intros.
+End TwoModules2.
 
-      - apply specializeMod_traceRefines_drop; auto.
+Section DuplicateTwoModules2.
+  Variables (m1 m2: nat -> Modules).
+  Hypotheses (Hsp1: forall iv, Specializable (m1 iv))
+             (Hsp2: forall iv, Specializable (m2 iv))
+             (Hequiv1: forall iv, ModEquiv type typeUT (m1 iv))
+             (Hequiv2: forall iv, ModEquiv type typeUT (m2 iv))
+             (Hvr1: forall iv, ValidRegsModules type (m1 iv))
+             (Hvr2: forall iv, ValidRegsModules type (m2 iv)).
 
-      - apply traceRefines_modular_noninteracting_p; auto.
-        + apply specializeMod_ModEquiv; auto.
-        + apply specializeMod_ModEquiv; auto.
-        + apply duplicate_ModEquiv; auto.
-        + apply duplicate_ModEquiv; auto.
-        + apply duplicate_specializeMod_disj_regs; auto.
-        + apply duplicate_specializeMod_disj_regs; auto.
-        + pose proof (duplicate_validRegsModules m1 (S n) Hvr1); auto.
-        + pose proof (duplicate_validRegsModules m2 (S n) Hvr2); auto.
-        + apply duplicate_specializeMod_disj_defs; auto.
-        + apply duplicate_specializeMod_disj_calls; auto.
-        + apply duplicate_specializeMod_disj_defs; auto.
-        + apply duplicate_specializeMod_disj_calls; auto.
-        + split.
-          * apply equivalentLabelMapElem_dropI_dropN; omega.
-          * apply equivalentLabelMapElem_dropN_dropI; omega.
-        + apply duplicate_noninteracting; auto.
-        + apply duplicate_noninteracting; auto.
-        + apply specializeMod_traceRefines_drop; auto.
-    Qed.
+  Variable (ds: string). (* a single label to drop *)
 
-  End TwoModules2.
+  Hypothesis (Hexts: forall iv1 iv2,
+                 SubList (filter (fun s => negb (string_eq s ds))
+                                 (getExtMeths (m1 iv1)))
+                         (getExtMeths (m2 iv2))).
+  
+  Lemma equivalentLabelMapElem_dropN_dropI:
+    forall n u (Ht: u > n),
+      EquivalentLabelMapElem (dropN ds n) (compLabelMaps (dropI ds u) (dropN ds n))
+                             (getExtMeths (duplicate m1 n)).
+  Proof.
+    induction n; unfold EquivalentLabelMapElem; intros.
+    - simpl; unfold compLabelMaps, dropI.
+      destruct (string_eq _ (ds __ 0)); auto.
+      remember (string_eq _ _) as st; destruct st; auto.
+      apply string_eq_dec_eq in Heqst; subst.
+      simpl in H.
+      apply spDom_getExtMeths in H.
+      apply specializeMod_dom_indexed in H; auto; dest.
+      apply withIndex_index_eq in H; dest; omega.
+    - simpl; assert (u > n) by omega; specialize (IHn _ H0); clear H0.
+      simpl in H.
+      apply getExtMeths_in in H; destruct H.
+      + clear IHn.
+        unfold dropI, compLabelMaps.
+        destruct (dropN ds n s v); auto.
+        destruct (string_eq _ (ds __ (S n))); auto.
+        remember (string_eq _ _) as st; destruct st; auto.
+        exfalso; apply string_eq_dec_eq in Heqst; subst.
+        apply spDom_getExtMeths in H.
+        apply specializeMod_dom_indexed in H; auto; dest.
+        apply withIndex_index_eq in H; dest; omega.
+      + unfold compLabelMaps.
+        rewrite IHn; clear IHn; auto.
+        unfold compLabelMaps.
+        destruct (dropN ds n s v); auto.
+        destruct (dropI ds u s s0); auto.
+        destruct (dropI ds (S n) s s1); auto.
+        unfold dropI; remember (string_eq _ _) as st; destruct st; auto.
+        exfalso; apply string_eq_dec_eq in Heqst; subst.
+        apply spDom_getExtMeths in H.
+        apply duplicate_dom_indexed in H; auto; dest.
+        apply withIndex_index_eq in H; dest; omega.
+  Qed.
 
-  Section TwoModules3.
-    Variables (m1 m2: Modules).
-    Hypotheses (Hequiv1: forall ty, ModEquiv ty typeUT m1)
-               (Hequiv2: forall ty, ModEquiv ty typeUT m2)
-               (Hvr1: forall ty, ValidRegsModules ty m1)
-               (Hvr2: forall ty, ValidRegsModules ty m2)
-               (Hsp1: Specializable m1)
-               (Hsp2: Specializable m2).
+  Lemma duplicate_traceRefines_drop:
+    forall n,
+      (forall i, (m1 i) <<=[dropP ds] (m2 i)) ->
+      (duplicate m1 n <<=[dropN ds n] duplicate m2 n).
+  Proof.
+    induction n; simpl; intros.
+    - apply specializeMod_traceRefines_drop; auto.
+    - apply traceRefines_modular_noninteracting_p; auto.
+      + apply specializeMod_ModEquiv; auto.
+      + apply specializeMod_ModEquiv; auto.
+      + apply duplicate_ModEquiv; auto.
+      + apply duplicate_ModEquiv; auto.
+      + apply duplicate_specializeMod_disj_regs; auto.
+      + apply duplicate_specializeMod_disj_regs; auto.
+      + pose proof (duplicate_validRegsModules m1 (S n) Hvr1); auto.
+      + pose proof (duplicate_validRegsModules m2 (S n) Hvr2); auto.
+      + apply duplicate_specializeMod_disj_defs; auto.
+      + apply duplicate_specializeMod_disj_calls; auto.
+      + apply duplicate_specializeMod_disj_defs; auto.
+      + apply duplicate_specializeMod_disj_calls; auto.
+      + split.
+        * apply equivalentLabelMapElem_dropI_dropN; auto; omega.
+        * apply equivalentLabelMapElem_dropN_dropI; auto; omega.
+      + apply duplicate_noninteracting; auto.
+      + apply duplicate_noninteracting; auto.
+      + apply specializeMod_traceRefines_drop; auto.
+  Qed.
 
-    Lemma duplicate_regs_ConcatMod_1:
-      forall n,
-        SubList (getRegInits (duplicate (m1 ++ m2)%kami n))
-                (getRegInits (duplicate m1 n ++ duplicate m2 n)%kami).
-    Proof.
-      Opaque specializeMod.
-      induction n; intros.
-      - unfold duplicate.
-        rewrite specializeMod_concatMod; auto.
-        apply SubList_refl.
-      - simpl in *; apply SubList_app_3.
-        + rewrite specializeMod_concatMod; auto.
-          simpl; apply SubList_app_3.
-          * do 2 apply SubList_app_1; apply SubList_refl.
-          * apply SubList_app_2, SubList_app_1, SubList_refl.
-        + unfold SubList in *; intros.
-          specialize (IHn e H).
-          apply in_app_or in IHn; destruct IHn.
-          * apply in_or_app; left; apply in_or_app; auto.
-          * apply in_or_app; right; apply in_or_app; auto.
-            Transparent specializeMod.
-    Qed.
+End DuplicateTwoModules2.
 
-    Lemma duplicate_regs_ConcatMod_2:
-      forall n,
-        SubList (getRegInits (duplicate m1 n ++ duplicate m2 n)%kami)
-                (getRegInits (duplicate (m1 ++ m2)%kami n)).
-    Proof.
-      Opaque specializeMod.
-      induction n; intros.
-      - unfold duplicate.
-        rewrite specializeMod_concatMod; auto.
-        apply SubList_refl.
-      - simpl in *; apply SubList_app_3.
-        + rewrite specializeMod_concatMod; auto.
-          simpl; apply SubList_app_3.
-          * do 2 apply SubList_app_1; apply SubList_refl.
-          * apply SubList_app_2; apply SubList_app_4 in IHn; auto.
-        + rewrite specializeMod_concatMod; auto.
-          simpl; apply SubList_app_3.
-          * apply SubList_app_1, SubList_app_2, SubList_refl.
-          * apply SubList_app_2; apply SubList_app_5 in IHn; auto.
-            Transparent specializeMod.
-    Qed.
+Section DuplicateTwoModules3.
+  Variables (m1 m2: nat -> Modules).
+  Hypotheses (Hequiv1: forall iv ty, ModEquiv ty typeUT (m1 iv))
+             (Hequiv2: forall iv ty, ModEquiv ty typeUT (m2 iv))
+             (Hvr1: forall iv ty, ValidRegsModules ty (m1 iv))
+             (Hvr2: forall iv ty, ValidRegsModules ty (m2 iv))
+             (Hsp1: forall iv, Specializable (m1 iv))
+             (Hsp2: forall iv, Specializable (m2 iv)).
 
-    Corollary duplicate_regs_ConcatMod:
-      forall n,
-        EquivList (getRegInits (duplicate m1 n ++ duplicate m2 n)%kami)
-                  (getRegInits (duplicate (m1 ++ m2)%kami n)).
-    Proof.
-      intros; split.
-      - apply duplicate_regs_ConcatMod_2.
-      - apply duplicate_regs_ConcatMod_1.
-    Qed.
+  Lemma duplicate_regs_ConcatMod_1:
+    forall n,
+      SubList (getRegInits (duplicate (fun i => (m1 i) ++ (m2 i))%kami n))
+              (getRegInits (duplicate m1 n ++ duplicate m2 n)%kami).
+  Proof.
+    Opaque specializeMod.
+    induction n; intros.
+    - unfold duplicate.
+      rewrite specializeMod_concatMod; auto.
+      apply SubList_refl.
+    - simpl in *; apply SubList_app_3.
+      + rewrite specializeMod_concatMod; auto.
+        simpl; apply SubList_app_3.
+        * do 2 apply SubList_app_1; apply SubList_refl.
+        * apply SubList_app_2, SubList_app_1, SubList_refl.
+      + unfold SubList in *; intros.
+        specialize (IHn e H).
+        apply in_app_or in IHn; destruct IHn.
+        * apply in_or_app; left; apply in_or_app; auto.
+        * apply in_or_app; right; apply in_or_app; auto.
+          Transparent specializeMod.
+  Qed.
 
-    Lemma duplicate_regs_NoDup_2:
-      NoDup (namesOf (getRegInits (m1 ++ m2)%kami)) ->
-      forall n,
-        NoDup (namesOf (getRegInits (duplicate m1 n ++ duplicate m2 n)%kami)).
-    Proof.
-      Opaque specializeMod.
-      intros.
-      pose proof H; apply duplicate_regs_NoDup with (n:= n) in H0.
-      induction n; simpl; intros.
-      - simpl in *; rewrite specializeMod_concatMod in H0; auto.
-      - assert (NoDup (namesOf (getRegInits (duplicate (m1 ++ m2)%kami n)))).
-        { apply duplicate_regs_NoDup; auto.
-          apply specializable_concatMod; auto.
-        }
-        specialize (IHn H1); clear H1.
-        unfold namesOf; repeat rewrite map_app.
-        rewrite app_assoc.
-        rewrite <-app_assoc with (l:= map (@attrName _) (getRegInits (specializeMod m1 (S n)))).
-        rewrite <-app_assoc with (l:= map (@attrName _) (getRegInits (specializeMod m1 (S n)))).
-        apply NoDup_app_comm_ext.
-        rewrite app_assoc.
-        rewrite app_assoc.
-        rewrite <-app_assoc with (n:= map (@attrName _) (getRegInits (duplicate m2 n))).
-        apply NoDup_DisjList.
-        + apply specializeMod_regs_NoDup with (i:= S n) in H;
-            [|apply specializable_concatMod; auto].
-          rewrite specializeMod_concatMod in H; auto.
-          rewrite <-map_app; auto.
-        + rewrite <-map_app; auto.
-        + do 2 rewrite <-map_app.
-          pose proof (duplicate_regs_ConcatMod_2 n).
-          apply SubList_map with (f:= @attrName _) in H1.
-          eapply DisjList_comm, DisjList_SubList; eauto.
-          pose proof (specializeMod_concatMod Hvr1 Hvr2 Hequiv1 Hequiv2 (S n) Hsp1 Hsp2).
-          change (getRegInits (specializeMod m1 (S n)) ++ getRegInits (specializeMod m2 (S n)))
-          with (getRegInits (specializeMod m1 (S n) ++ (specializeMod m2 (S n)))%kami).
-          rewrite <-H2.
-          apply DisjList_comm, duplicate_specializeMod_disj_regs; auto.
-          apply specializable_concatMod; auto.
-      - apply specializable_concatMod; auto.
-    Qed.
+  Lemma duplicate_regs_ConcatMod_2:
+    forall n,
+      SubList (getRegInits (duplicate m1 n ++ duplicate m2 n)%kami)
+              (getRegInits (duplicate (fun i => m1 i ++ m2 i)%kami n)).
+  Proof.
+    Opaque specializeMod.
+    induction n; intros.
+    - unfold duplicate.
+      rewrite specializeMod_concatMod; auto.
+      apply SubList_refl.
+    - simpl in *; apply SubList_app_3.
+      + rewrite specializeMod_concatMod; auto.
+        simpl; apply SubList_app_3.
+        * do 2 apply SubList_app_1; apply SubList_refl.
+        * apply SubList_app_2; apply SubList_app_4 in IHn; auto.
+      + rewrite specializeMod_concatMod; auto.
+        simpl; apply SubList_app_3.
+        * apply SubList_app_1, SubList_app_2, SubList_refl.
+        * apply SubList_app_2; apply SubList_app_5 in IHn; auto.
+          Transparent specializeMod.
+  Qed.
 
-    Lemma duplicate_rules_ConcatMod_1:
-      forall n,
-        SubList (getRules (duplicate (m1 ++ m2)%kami n))
-                (getRules (duplicate m1 n ++ duplicate m2 n)%kami).
-    Proof.
-      Opaque specializeMod.
-      induction n; intros.
-      - unfold duplicate.
-        rewrite specializeMod_concatMod; auto.
-        apply SubList_refl.
-      - simpl in *; apply SubList_app_3.
-        + rewrite specializeMod_concatMod; auto.
-          simpl; apply SubList_app_3.
-          * do 2 apply SubList_app_1; apply SubList_refl.
-          * apply SubList_app_2, SubList_app_1, SubList_refl.
-        + unfold SubList in *; intros.
-          specialize (IHn e H).
-          apply in_app_or in IHn; destruct IHn.
-          * apply in_or_app; left; apply in_or_app; auto.
-          * apply in_or_app; right; apply in_or_app; auto.
-            Transparent specializeMod.
-    Qed.
+  Corollary duplicate_regs_ConcatMod:
+    forall n,
+      EquivList (getRegInits (duplicate m1 n ++ duplicate m2 n)%kami)
+                (getRegInits (duplicate (fun i => m1 i ++ m2 i)%kami n)).
+  Proof.
+    intros; split.
+    - apply duplicate_regs_ConcatMod_2.
+    - apply duplicate_regs_ConcatMod_1.
+  Qed.
 
-    Lemma duplicate_rules_ConcatMod_2:
-      forall n,
-        SubList (getRules (duplicate m1 n ++ duplicate m2 n)%kami)
-                (getRules (duplicate (m1 ++ m2)%kami n)).
-    Proof.
-      Opaque specializeMod.
-      induction n; intros.
-      - unfold duplicate.
-        rewrite specializeMod_concatMod; auto.
-        apply SubList_refl.
-      - simpl in *; apply SubList_app_3.
-        + rewrite specializeMod_concatMod; auto.
-          simpl; apply SubList_app_3.
-          * do 2 apply SubList_app_1; apply SubList_refl.
-          * apply SubList_app_2; apply SubList_app_4 in IHn; auto.
-        + rewrite specializeMod_concatMod; auto.
-          simpl; apply SubList_app_3.
-          * apply SubList_app_1, SubList_app_2, SubList_refl.
-          * apply SubList_app_2; apply SubList_app_5 in IHn; auto.
-            Transparent specializeMod.
-    Qed.
+  Lemma duplicate_regs_NoDup_2:
+    (forall i, NoDup (namesOf (getRegInits (m1 i ++ m2 i)%kami))) ->
+    forall n,
+      NoDup (namesOf (getRegInits (duplicate m1 n ++ duplicate m2 n)%kami)).
+  Proof.
+    Opaque specializeMod.
+    intros.
+    pose proof H; apply duplicate_regs_NoDup with (n:= n) in H0.
+    induction n; simpl; intros.
+    - simpl in *; rewrite specializeMod_concatMod in H0; auto.
+    - assert (NoDup (namesOf (getRegInits (duplicate (fun i => m1 i ++ m2 i)%kami n)))).
+      { apply duplicate_regs_NoDup; auto.
+        intros; apply specializable_concatMod; auto.
+      }
+      specialize (IHn H1); clear H1.
+      unfold namesOf; repeat rewrite map_app.
+      rewrite app_assoc.
+      rewrite <-app_assoc with (l:= map (@attrName _)
+                                        (getRegInits (specializeMod (m1 (S n)) (S n)))).
+      rewrite <-app_assoc with (l:= map (@attrName _)
+                                        (getRegInits (specializeMod (m1 (S n)) (S n)))).
+      apply NoDup_app_comm_ext.
+      rewrite app_assoc.
+      rewrite app_assoc.
+      rewrite <-app_assoc with (n:= map (@attrName _) (getRegInits (duplicate m2 n))).
+      apply NoDup_DisjList.
+      + specialize (H (S n)); apply specializeMod_regs_NoDup with (i:= S n) in H;
+          [|apply specializable_concatMod; auto].
+        rewrite specializeMod_concatMod in H; auto.
+        rewrite <-map_app; auto.
+      + rewrite <-map_app; auto.
+      + do 2 rewrite <-map_app.
+        pose proof (duplicate_regs_ConcatMod_2 n).
+        apply SubList_map with (f:= @attrName _) in H1.
+        eapply DisjList_comm, DisjList_SubList; eauto.
+        pose proof (specializeMod_concatMod (Hvr1 (S n)) (Hvr2 (S n))
+                                            (Hequiv1 (S n)) (Hequiv2 (S n)) (S n)
+                                            (Hsp1 (S n)) (Hsp2 (S n))).
+        change (getRegInits (specializeMod (m1 (S n)) (S n)) ++
+                            getRegInits (specializeMod (m2 (S n)) (S n)))
+        with (getRegInits (specializeMod (m1 (S n)) (S n) ++
+                                         (specializeMod (m2 (S n)) (S n)))%kami).
+        rewrite <-H2.
+        apply DisjList_comm.
+        change (m1 (S n) ++ m2 (S n))%kami with ((fun i => (m1 i ++ m2 i)%kami) (S n)).
+        apply duplicate_specializeMod_disj_regs; auto.
+        intros; apply specializable_concatMod; auto.
+    - intros; apply specializable_concatMod; auto.
+  Qed.
 
-    Corollary duplicate_rules_ConcatMod:
-      forall n,
-        EquivList (getRules (duplicate m1 n ++ duplicate m2 n)%kami)
-                  (getRules (duplicate (m1 ++ m2)%kami n)).
-    Proof.
-      intros; split.
-      - apply duplicate_rules_ConcatMod_2.
-      - apply duplicate_rules_ConcatMod_1.
-    Qed.
+  Lemma duplicate_rules_ConcatMod_1:
+    forall n,
+      SubList (getRules (duplicate (fun i => m1 i ++ m2 i)%kami n))
+              (getRules (duplicate m1 n ++ duplicate m2 n)%kami).
+  Proof.
+    Opaque specializeMod.
+    induction n; intros.
+    - unfold duplicate.
+      rewrite specializeMod_concatMod; auto.
+      apply SubList_refl.
+    - simpl in *; apply SubList_app_3.
+      + rewrite specializeMod_concatMod; auto.
+        simpl; apply SubList_app_3.
+        * do 2 apply SubList_app_1; apply SubList_refl.
+        * apply SubList_app_2, SubList_app_1, SubList_refl.
+      + unfold SubList in *; intros.
+        specialize (IHn e H).
+        apply in_app_or in IHn; destruct IHn.
+        * apply in_or_app; left; apply in_or_app; auto.
+        * apply in_or_app; right; apply in_or_app; auto.
+          Transparent specializeMod.
+  Qed.
 
-    Lemma duplicate_defs_ConcatMod_1:
-      forall n,
-        SubList (getDefsBodies (duplicate (m1 ++ m2)%kami n))
-                (getDefsBodies (duplicate m1 n ++ duplicate m2 n)%kami).
-    Proof.
-      Opaque specializeMod.
-      induction n; intros.
-      - unfold duplicate.
-        rewrite specializeMod_concatMod; auto.
-        apply SubList_refl.
-      - simpl in *; apply SubList_app_3.
-        + rewrite specializeMod_concatMod; auto.
-          simpl; apply SubList_app_3.
-          * do 2 apply SubList_app_1; apply SubList_refl.
-          * apply SubList_app_2, SubList_app_1, SubList_refl.
-        + unfold SubList in *; intros.
-          specialize (IHn e H).
-          apply in_app_or in IHn; destruct IHn.
-          * apply in_or_app; left; apply in_or_app; auto.
-          * apply in_or_app; right; apply in_or_app; auto.
-            Transparent specializeMod.
-    Qed.
+  Lemma duplicate_rules_ConcatMod_2:
+    forall n,
+      SubList (getRules (duplicate m1 n ++ duplicate m2 n)%kami)
+              (getRules (duplicate (fun i => m1 i ++ m2 i)%kami n)).
+  Proof.
+    Opaque specializeMod.
+    induction n; intros.
+    - unfold duplicate.
+      rewrite specializeMod_concatMod; auto.
+      apply SubList_refl.
+    - simpl in *; apply SubList_app_3.
+      + rewrite specializeMod_concatMod; auto.
+        simpl; apply SubList_app_3.
+        * do 2 apply SubList_app_1; apply SubList_refl.
+        * apply SubList_app_2; apply SubList_app_4 in IHn; auto.
+      + rewrite specializeMod_concatMod; auto.
+        simpl; apply SubList_app_3.
+        * apply SubList_app_1, SubList_app_2, SubList_refl.
+        * apply SubList_app_2; apply SubList_app_5 in IHn; auto.
+          Transparent specializeMod.
+  Qed.
 
-    Lemma duplicate_defs_ConcatMod_2:
-      forall n,
-        SubList (getDefsBodies (duplicate m1 n ++ duplicate m2 n)%kami)
-                (getDefsBodies (duplicate (m1 ++ m2)%kami n)).
-    Proof.
-      Opaque specializeMod.
-      induction n; intros.
-      - unfold duplicate.
-        rewrite specializeMod_concatMod; auto.
-        apply SubList_refl.
-      - simpl in *; apply SubList_app_3.
-        + rewrite specializeMod_concatMod; auto.
-          simpl; apply SubList_app_3.
-          * do 2 apply SubList_app_1; apply SubList_refl.
-          * apply SubList_app_2; apply SubList_app_4 in IHn; auto.
-        + rewrite specializeMod_concatMod; auto.
-          simpl; apply SubList_app_3.
-          * apply SubList_app_1, SubList_app_2, SubList_refl.
-          * apply SubList_app_2; apply SubList_app_5 in IHn; auto.
-            Transparent specializeMod.
-    Qed.
+  Corollary duplicate_rules_ConcatMod:
+    forall n,
+      EquivList (getRules (duplicate m1 n ++ duplicate m2 n)%kami)
+                (getRules (duplicate (fun i => m1 i ++ m2 i)%kami n)).
+  Proof.
+    intros; split.
+    - apply duplicate_rules_ConcatMod_2.
+    - apply duplicate_rules_ConcatMod_1.
+  Qed.
 
-    Lemma duplicate_defs_ConcatMod:
-      forall n,
-        EquivList (getDefsBodies (duplicate m1 n ++ duplicate m2 n)%kami)
-                  (getDefsBodies (duplicate (m1 ++ m2)%kami n)).
-    Proof.
-      intros; split.
-      - apply duplicate_defs_ConcatMod_2.
-      - apply duplicate_defs_ConcatMod_1.
-    Qed.
+  Lemma duplicate_defs_ConcatMod_1:
+    forall n,
+      SubList (getDefsBodies (duplicate (fun i => m1 i ++ m2 i)%kami n))
+              (getDefsBodies (duplicate m1 n ++ duplicate m2 n)%kami).
+  Proof.
+    Opaque specializeMod.
+    induction n; intros.
+    - unfold duplicate.
+      rewrite specializeMod_concatMod; auto.
+      apply SubList_refl.
+    - simpl in *; apply SubList_app_3.
+      + rewrite specializeMod_concatMod; auto.
+        simpl; apply SubList_app_3.
+        * do 2 apply SubList_app_1; apply SubList_refl.
+        * apply SubList_app_2, SubList_app_1, SubList_refl.
+      + unfold SubList in *; intros.
+        specialize (IHn e H).
+        apply in_app_or in IHn; destruct IHn.
+        * apply in_or_app; left; apply in_or_app; auto.
+        * apply in_or_app; right; apply in_or_app; auto.
+          Transparent specializeMod.
+  Qed.
 
-  End TwoModules3.
+  Lemma duplicate_defs_ConcatMod_2:
+    forall n,
+      SubList (getDefsBodies (duplicate m1 n ++ duplicate m2 n)%kami)
+              (getDefsBodies (duplicate (fun i => m1 i ++ m2 i)%kami n)).
+  Proof.
+    Opaque specializeMod.
+    induction n; intros.
+    - unfold duplicate.
+      rewrite specializeMod_concatMod; auto.
+      apply SubList_refl.
+    - simpl in *; apply SubList_app_3.
+      + rewrite specializeMod_concatMod; auto.
+        simpl; apply SubList_app_3.
+        * do 2 apply SubList_app_1; apply SubList_refl.
+        * apply SubList_app_2; apply SubList_app_4 in IHn; auto.
+      + rewrite specializeMod_concatMod; auto.
+        simpl; apply SubList_app_3.
+        * apply SubList_app_1, SubList_app_2, SubList_refl.
+        * apply SubList_app_2; apply SubList_app_5 in IHn; auto.
+          Transparent specializeMod.
+  Qed.
 
-  Section TwoModules4.
-    Variables (m1 m2: Modules).
-    Hypotheses (Hsp1: Specializable m1)
-               (Hsp2: Specializable m2)
-               (Hvr1: forall ty, ValidRegsModules ty m1)
-               (Hvr2: forall ty, ValidRegsModules ty m2)
-               (Hequiv1: forall ty, ModEquiv ty typeUT m1)
-               (Hequiv2: forall ty, ModEquiv ty typeUT m2)
-               (HnoDup: NoDup (namesOf (getRegInits (m1 ++ m2)%kami))).
+  Lemma duplicate_defs_ConcatMod:
+    forall n,
+      EquivList (getDefsBodies (duplicate m1 n ++ duplicate m2 n)%kami)
+                (getDefsBodies (duplicate (fun i => m1 i ++ m2 i)%kami n)).
+  Proof.
+    intros; split.
+    - apply duplicate_defs_ConcatMod_2.
+    - apply duplicate_defs_ConcatMod_1.
+  Qed.
 
-    Lemma duplicate_concatMod_comm_1:
-      forall n,
-        duplicate (m1 ++ m2)%kami n <<== ((duplicate m1 n) ++ (duplicate m2 n))%kami.
-    Proof.
-      intros; rewrite idElementwiseId.
-      apply traceRefines_same_module_structure.
-      - apply duplicate_regs_NoDup; auto.
-        apply specializable_concatMod; auto.
-      - apply duplicate_regs_NoDup_2; auto.
-      - split.
-        + apply duplicate_regs_ConcatMod_1; auto.
-        + apply duplicate_regs_ConcatMod_2; auto.
-      - split.
-        + apply duplicate_rules_ConcatMod_1; auto.
-        + apply duplicate_rules_ConcatMod_2; auto.
-      - split.
-        + apply duplicate_defs_ConcatMod_1; auto.
-        + apply duplicate_defs_ConcatMod_2; auto.
-    Qed.
+End DuplicateTwoModules3.
 
-    Lemma duplicate_concatMod_comm_2:
-      forall n,
-        ((duplicate m1 n) ++ (duplicate m2 n))%kami <<== duplicate (m1 ++ m2)%kami n.
-    Proof.
-      intros; rewrite idElementwiseId.
-      apply traceRefines_same_module_structure.
-      - apply duplicate_regs_NoDup_2; auto.
-      - apply duplicate_regs_NoDup; auto.
-        apply specializable_concatMod; auto.
-      - split.
-        + apply duplicate_regs_ConcatMod_2; auto.
-        + apply duplicate_regs_ConcatMod_1; auto.
-      - split.
-        + apply duplicate_rules_ConcatMod_2; auto.
-        + apply duplicate_rules_ConcatMod_1; auto.
-      - split.
-        + apply duplicate_defs_ConcatMod_2; auto.
-        + apply duplicate_defs_ConcatMod_1; auto.
-    Qed.
+Section DuplicateTwoModules4.
+  Variables (m1 m2: nat -> Modules).
+  Hypotheses (Hsp1: forall iv, Specializable (m1 iv))
+             (Hsp2: forall iv, Specializable (m2 iv))
+             (Hequiv1: forall iv ty, ModEquiv ty typeUT (m1 iv))
+             (Hequiv2: forall iv ty, ModEquiv ty typeUT (m2 iv))
+             (Hvr1: forall iv ty, ValidRegsModules ty (m1 iv))
+             (Hvr2: forall iv ty, ValidRegsModules ty (m2 iv))
+             (HnoDup: forall iv, NoDup (namesOf (getRegInits (m1 iv ++ m2 iv)%kami))).
 
-  End TwoModules4.
+  Lemma duplicate_concatMod_comm_1:
+    forall n,
+      duplicate (fun i => m1 i ++ m2 i)%kami n <<== ((duplicate m1 n) ++ (duplicate m2 n))%kami.
+  Proof.
+    intros; rewrite idElementwiseId.
+    apply traceRefines_same_module_structure.
+    - apply duplicate_regs_NoDup; auto.
+      intros; apply specializable_concatMod; auto.
+    - apply duplicate_regs_NoDup_2; auto.
+    - split.
+      + apply duplicate_regs_ConcatMod_1; auto.
+      + apply duplicate_regs_ConcatMod_2; auto.
+    - split.
+      + apply duplicate_rules_ConcatMod_1; auto.
+      + apply duplicate_rules_ConcatMod_2; auto.
+    - split.
+      + apply duplicate_defs_ConcatMod_1; auto.
+      + apply duplicate_defs_ConcatMod_2; auto.
+  Qed.
 
-End DuplicateFacts.
+  Lemma duplicate_concatMod_comm_2:
+    forall n,
+      ((duplicate m1 n) ++ (duplicate m2 n))%kami <<== duplicate (fun i => m1 i ++ m2 i)%kami n.
+  Proof.
+    intros; rewrite idElementwiseId.
+    apply traceRefines_same_module_structure.
+    - apply duplicate_regs_NoDup_2; auto.
+    - apply duplicate_regs_NoDup; auto.
+      intros; apply specializable_concatMod; auto.
+    - split.
+      + apply duplicate_regs_ConcatMod_2; auto.
+      + apply duplicate_regs_ConcatMod_1; auto.
+    - split.
+      + apply duplicate_rules_ConcatMod_2; auto.
+      + apply duplicate_rules_ConcatMod_1; auto.
+    - split.
+      + apply duplicate_defs_ConcatMod_2; auto.
+      + apply duplicate_defs_ConcatMod_1; auto.
+  Qed.
+
+End DuplicateTwoModules4.
 
 Hint Unfold specializeMod duplicate: ModuleDefs.
 
