extraction/Extraction.v
@@ -1,7 +1,7 @@
 Require Import List String.
 Require Import Lib.Word Kami.Syntax Kami.Semantics Kami.Duplicate
         Kami.Notations Kami.Synthesize Ex.IsaRv32 Ex.IsaRv32Pgm.
-Require Import Ex.ProcFetchDecode Ex.ProcThreeStage Ex.ProcFourStDec.
+Require Import Ex.SC Ex.ProcFetchDecode Ex.ProcThreeStage Ex.ProcFourStDec.
 Require Import Ex.MemTypes Ex.MemAtomic Ex.MemCorrect Ex.ProcMemCorrect.
 Require Import Ext.BSyntax.
 
@@ -12,7 +12,9 @@ Set Extraction Optimize.
 Set Extraction KeepSingleton.
 Unset Extraction AutoInline.
 
-(** p4st + pmFifos ++ memCache extraction *)
+(** * p4st + pmFifos ++ memCache extraction *)
+
+(** Some numbers *)
 
 (* (idxBits + tagBits + lgNumDatas) should be equal to rv32iAddrSize (= 16) *)
 Definition idxBits := 8.
@@ -22,46 +24,8 @@ Definition lgNumChildren := 2. (* 2^2 = 4 cores *)
 Definition fifoSize := 2.
 Definition idK := Bit 1.
 
-Definition predictNextPc ty (ppc: fullType ty (SyntaxKind (Bit rv32iAddrSize))) :=
-  (#ppc + $4)%kami_expr.
-
-Definition p4stNMemCache :=
-  ProcMemCorrect.p4stNMemCache
-    fifoSize idxBits tagBits lgNumDatas idK
-    rv32iGetOptype rv32iGetLdDst rv32iGetLdAddr rv32iGetLdSrc rv32iCalcLdAddr
-    rv32iGetStAddr rv32iGetStSrc rv32iCalcStAddr rv32iGetStVSrc
-    rv32iGetSrc1 rv32iGetSrc2 rv32iGetDst rv32iExec rv32iNextPc
-    rv32iAlignPc rv32iAlignAddr predictNextPc lgNumChildren.
-
-(** * The correctness of the extraction target is proven! Trust us! *)
-Section Correctness.
-
-  (* Spec: sequential consistency for multicore *)
-  Definition scN :=
-    ProcMemCorrect.scN
-      idxBits tagBits lgNumDatas
-      rv32iGetOptype rv32iGetLdDst rv32iGetLdAddr rv32iGetLdSrc rv32iCalcLdAddr
-      rv32iGetStAddr rv32iGetStSrc rv32iCalcStAddr rv32iGetStVSrc
-      rv32iGetSrc1 rv32iGetSrc2 rv32iGetDst rv32iExec rv32iNextPc
-      rv32iAlignPc rv32iAlignAddr lgNumChildren.
-
-  Theorem p4stNMemCache_refines_scN: p4stNMemCache <<== scN.
-  Proof.
-    apply p4stN_mcache_refines_scN.
-  Qed.
-
-End Correctness.
-
-(** targetPgms should be your target program *)
-Require Import Ex.IsaRv32PgmExt.
-Definition targetPgms :=
-  IsaRv32PgmBankerInit.pgmExt
-    :: IsaRv32PgmBankerWorker1.pgmExt
-    :: IsaRv32PgmBankerWorker2.pgmExt
-    :: IsaRv32PgmBankerWorker3.pgmExt :: nil.
-
-(** targetM should be your target module *)
-Definition targetProcM := p4stNMemCache.
+(** Some initial values *)
+Eval compute in ((numChildren lgNumChildren) + 1).
 
 (* A utility function for setting the stack pointer in rf *)
 Definition rfWithSpInit (sp: ConstT (Data rv32iDataBytes))
@@ -85,30 +49,59 @@ Definition rfWithSpInit (sp: ConstT (Data rv32iDataBytes))
     exact $0.
 Defined.
 
-(** targetRfs should be a list of initial values of processors' register files *)
-Definition targetRfs : list (ConstT (Vector (Data rv32iDataBytes) rv32iRfIdx)) :=
-  (rfWithSpInit (ConstBit (natToWord _ 64)))
-    :: (rfWithSpInit (ConstBit (natToWord _ 128)))
-    :: (rfWithSpInit (ConstBit (natToWord _ 192)))
-    :: (rfWithSpInit (ConstBit (natToWord _ 256)))
+Require Import Ex.IsaRv32PgmExt.
+
+Definition procInits : list (ProcInit rv32iAddrSize rv32iIAddrSize rv32iDataBytes rv32iRfIdx) :=
+  {| pcInit := Default;
+     rfInit := rfWithSpInit (ConstBit (natToWord _ 64));
+     pgmInit := IsaRv32PgmBankerInit.pgmExt |}
+    :: {| pcInit := Default;
+          rfInit := rfWithSpInit (ConstBit (natToWord _ 128));
+          pgmInit := IsaRv32PgmBankerWorker1.pgmExt |}
+    :: {| pcInit := Default;
+          rfInit := rfWithSpInit (ConstBit (natToWord _ 192));
+          pgmInit := IsaRv32PgmBankerWorker2.pgmExt |}
+    :: {| pcInit := Default;
+          rfInit := rfWithSpInit (ConstBit (natToWord _ 256));
+          pgmInit := IsaRv32PgmBankerWorker3.pgmExt |}
     :: nil.
 
+Definition predictNextPc ty (ppc: fullType ty (SyntaxKind (Bit rv32iAddrSize))) :=
+  (#ppc + $4)%kami_expr.
+
+Definition p4stNMemCache :=
+  ProcMemCorrect.p4stNMemCache
+    fifoSize idxBits tagBits lgNumDatas idK
+    rv32iGetOptype rv32iGetLdDst rv32iGetLdAddr rv32iGetLdSrc rv32iCalcLdAddr
+    rv32iGetStAddr rv32iGetStSrc rv32iCalcStAddr rv32iGetStVSrc
+    rv32iGetSrc1 rv32iGetSrc2 rv32iGetDst rv32iExec rv32iNextPc
+    rv32iAlignPc rv32iAlignAddr predictNextPc lgNumChildren procInits.
+
+(** * The correctness of the extraction target is proven! Trust us! *)
+Section Correctness.
+
+  (* Spec: sequential consistency for multicore *)
+  Definition scN :=
+    ProcMemCorrect.scN
+      idxBits tagBits lgNumDatas
+      rv32iGetOptype rv32iGetLdDst rv32iGetLdAddr rv32iGetLdSrc rv32iCalcLdAddr
+      rv32iGetStAddr rv32iGetStSrc rv32iCalcStAddr rv32iGetStVSrc
+      rv32iGetSrc1 rv32iGetSrc2 rv32iGetDst rv32iExec rv32iNextPc
+      rv32iAlignPc rv32iAlignAddr lgNumChildren procInits.
+
+  Theorem p4stNMemCache_refines_scN: p4stNMemCache <<== scN.
+  Proof.
+    apply p4stN_mcache_refines_scN.
+  Qed.
+
+End Correctness.
+
 (** DON'T REMOVE OR MODIFY BELOW LINES *)
+(* targetM should be your target module *)
+Definition targetProcM := p4stNMemCache.
 Definition targetProcS := getModuleS targetProcM.
 Definition targetProcB := ModulesSToBModules targetProcS.
 
-(* What to extract *)
-Record ExtTarget :=
-  { extPgms : list (ConstT (Vector (Data rv32iDataBytes) rv32iIAddrSize));
-    extProc : option (list BRegModule);
-    extRfs : list (ConstT (Vector (Data rv32iDataBytes) rv32iRfIdx))
-  }.
-
-Definition target : ExtTarget :=
-  {| extPgms := targetPgms;
-     extProc := targetProcB;
-     extRfs := targetRfs |}.
-
 (** Ocaml/Target.ml is used with Ocaml/PP.ml and Main.ml to build a converter to Bluespec. *)
-Extraction "./extraction/Ocaml/Target.ml" target.
+Extraction "./extraction/Ocaml/Target.ml" targetProcB.
 
